cvc5Test/Sanity.lean
@@ -1,0 +1,58 @@
+import cvc5Test.Init
+
+
+
+namespace cvc5.Test
+
+def testSort (getSort : Env cvc5.Sort) : IO Unit := do
+  let res ← Env.run do
+    let sort ← getSort
+    println! "sort := `{sort}`"
+  match res with
+  | .ok () => return ()
+  | .error e => IO.eprintln s!"ERROR\n{e}"
+
+/-- info: sort := `Bool` -/
+#guard_msgs in #eval testSort getBooleanSort
+/-- info: sort := `Int` -/
+#guard_msgs in #eval testSort getIntegerSort
+/-- info: sort := `Real` -/
+#guard_msgs in #eval testSort getRealSort
+/-- info: sort := `RegLan` -/
+#guard_msgs in #eval testSort getRegExpSort
+/-- info: sort := `RoundingMode` -/
+#guard_msgs in #eval testSort getRoundingModeSort
+/-- info: sort := `String` -/
+#guard_msgs in #eval testSort getStringSort
+
+/-- info: sort := `(Array Int String)` -/
+#guard_msgs in #eval testSort do
+  let int ← getIntegerSort
+  let string ← getStringSort
+  mkArraySort int string
+
+/-- info: sort := `(_ BitVec 5)` -/
+#guard_msgs in #eval testSort do
+  mkBitVectorSort 5
+
+/-- info: sort := `(_ FloatingPoint 10 10)` -/
+#guard_msgs in #eval testSort do
+  mkFloatingPointSort 10 10
+
+/-- info: sort := `(_ FiniteField 5)` -/
+#guard_msgs in #eval testSort do
+  mkFiniteFieldSortFromString "5" 10
+
+/-- info: sort := `(-> Int Real String String)` -/
+#guard_msgs in #eval testSort do
+  let int ← getIntegerSort
+  let real ← getRealSort
+  let string ← getStringSort
+  cvc5.mkFunctionSort #[int, real, string] string
+
+/-- info: sort := `(-> Int Real String Bool)` -/
+#guard_msgs in #eval testSort do
+  let int ← getIntegerSort
+  let real ← getRealSort
+  let string ← getStringSort
+  cvc5.mkPredicateSort #[int, real, string]
